Fix some strspn lemmas.

Examples/p32_addloop.v
@@ -2,6 +2,7 @@ Require Import NArith.
 Require Import ZArith.
 Require Import Picinae_pilbox32_interpreter.
 Require Import List.
+Require Import String.
 Import ListNotations.
 Open Scope N.
 
@@ -12,34 +13,10 @@ Definition addloop_program := [
   PIL_bne 0 2 (-8)%Z
 ].
 
-Definition p32_addloop: addr -> N :=
-  p32_assemble'' 0x00 addloop_program.
+(* Compute this then copy-paste into the file below. *)
+Compute print_code_prop addloop_program 0x00 "addloop_mem".
 
-
-(*Compute p32_assemble 0x00 addloop_program.
-echo "     = [(0, 1); (1, 0); (2, 0); (3, 0); (4, 134); (
-        5, 36); (6, 0); (7, 0); (8, 8); (9, 41); (
-        10, 0); (11, 0); (12, 18); (13, 8); (
-        14, 255); (15, 255)]" | tr '(' '|' | tr -d '=[)];' | sed 's/,/ =>/g; s/|/\n|/g'
-
-*)
-Definition p32_addloop' : addr -> N :=
-fun a => match a with
-|0 => 1 (*   PIL_li 0 0;  *)
-|1 => 0
-|2 => 0
-|3 => 0
-|4 => 134 (*   PIL_addi 1 1 1;  *)
-|5 => 36
-|6 => 0
-|7 => 0
-|8 => 8 (*   PIL_subi 2 2 1;  *)
-|9 => 41
-|10 => 0
-|11 => 0
-|12 => 22 (*   PIL_subi 2 2 1;  *)
-|13 => 8
-|14 => 255
-|15 => 255
-|_ => 0
-end.
+Definition addloop_mem (mem:N) : Prop :=
+ xbits mem 0 128 = 340277338626376526927524685974490578945.
+Definition addloop_mem_aexec (mem:N) : Prop :=
+  xbits mem 0 16 = 65535.
