Examples/p32_addloop_proofs.v
@@ -1,6 +1,7 @@
 Require Import NArith.
 Require Import ZArith.
 Require Import Picinae_pilbox32_interpreter.
+Require Import Lia.
 Import PIL32Notations.
 Require Import p32_addloop.
 
@@ -10,15 +11,15 @@ Definition add_loop_end   : N := 16.
 Section Invariants.
   Variables inp1 inp2 : N.
   Variable  s0 : store.
-  Hypothesis s_inp1 : s0 R_R1 = Ⓓ inp1.
-  Hypothesis s_inp2 : s0 R_R2 = Ⓓ inp2. 
+  Hypothesis s_inp1 : s0 R_R1 = inp1.
+  Hypothesis s_inp2 : s0 R_R2 = inp2. 
   
-  Definition postcondition (s:store) := s R_R1 = Ⓓ(inp1 ⊕ inp2).
+  Definition postcondition (s:store) := s R_R1 = (inp1 ⊕ inp2).
   Definition mem_unchanged (s:store) := s V_MEM32 = s0 V_MEM32 /\ s A_EXEC = s0 A_EXEC.
   Definition invs (t:trace) : option Prop:=
     match t with (Addr a, s) :: _ => match a with
-      | 0 => Some (s R_R1 = Ⓓ inp1 /\ s R_R2 = Ⓓ inp2 /\ mem_unchanged s)
-      | 4 => Some (exists r1 r2, s R_R0 = Ⓓ0 /\ s R_R1 = Ⓓr1 /\ s R_R2 = Ⓓr2
+      | 0 => Some (s R_R1 = inp1 /\ s R_R2 = inp2 /\ mem_unchanged s)
+      | 4 => Some (exists r1 r2, s R_R0 = 0 /\ s R_R1 = r1 /\ s R_R2 = r2
                                  /\ r1 ⊕ r2 = inp1 ⊕ inp2 /\ mem_unchanged s)
       | 16 => Some (postcondition s)
       | _ => None end
@@ -36,14 +37,18 @@ Definition exec_bits : addr -> N :=
   | 0 | 4 | 8 | 12 => 1
   | _ => 0 end.
 
+Theorem xbits_split2: forall i a b j x n : N,
+i <= a -> a <= b -> b <= j -> xbits x i j = n -> xbits x a b = xbits n (a-i) (b-i).
+Proof. Admitted.
+  
 Theorem addloop_correctness:
   forall s inp1 inp2 t s' x'
          (ENTRY: startof t (x',s') = (Addr 0,s))
          (MDL: models pil32typctx s)
-         (MEM: s V_MEM32 = Ⓜ p32_addloop')
-         (EXEC: s A_EXEC = Ⓜ exec_bits)
-         (INP1: s R_R1 = Ⓓinp1)
-         (INP2: s R_R2 = Ⓓinp2)
+         (MEM: addloop_mem (s V_MEM32))
+         (EXEC: addloop_mem_aexec (s A_EXEC))
+         (INP1: s R_R1 = inp1)
+         (INP2: s R_R2 = inp2)
 ,
 (* We define our program as p32_prog, a function that looks into
    a given store's memory and page-execute permissions to determine
@@ -72,11 +77,14 @@ Proof.
   clear - PRE MDL MEM EXEC. rename s into s0, t1 into t, s1 into s.
 
   destruct_inv 32 PRE.
-  destruct PRE as [IN1 [IN2 [MEMSAME EXECSAME]]]. unfold mem_unchanged in MEMSAME.
+  destruct PRE as [IN1 [IN2 [MEMSAME EXECSAME]]]. rewrite <-MEMSAME in MEM; rewrite <-EXECSAME in EXEC.
+
   step.
   exists inp1, inp2. repeat (split || trivial).
-  
+
   destruct PRE as [r1 [r2 [R0 [R1 [R2 [SUM [MEMSAME EXECSAME]]]]]]].
+  rewrite <-MEMSAME, <-EXECSAME in *.
+
   step. step. step.
   exists (1 ⊕ r1), (r2 ⊖ 1).
   rewrite Bool.negb_true_iff, N.eqb_neq in BC; unfold mem_unchanged.
