Examples/p32_dynamicli_proof.v
@@ -11,7 +11,7 @@ Section Invariants.
   Variables inp1 inp2 : N.
   Variable  s0 : store.
   
-  Definition postcondition (s:store) := s R_R5 = Ⓓ(777).
+  Definition postcondition (s:store) := s R_R5 = (777).
   Definition mem_unchanged (s:store) := s V_MEM32 = s0 V_MEM32 /\ s A_EXEC = s0 A_EXEC.
   Definition invs (t:trace) : option Prop:=
     match t with (Addr a, s) :: _ => match a with
@@ -36,8 +36,8 @@ Theorem dynamicli_correctness:
   forall s t s' x'
          (ENTRY: startof t (x',s') = (Addr 0,s))
          (MDL: models pil32typctx s)
-         (MEM: s V_MEM32 = Ⓜ p32_dynamicli')
-         (EXEC: s A_EXEC = Ⓜ exec_bits)
+         (MEM: dynamic_li (s V_MEM32))
+         (EXEC: dynamic_li_aexec (s A_EXEC))
 ,
 (* We define our program as p32_prog, a function that looks into
    a given store's memory and page-execute permissions to determine
@@ -67,9 +67,133 @@ intros. unfold satisfies_all.
 
   destruct_inv 32 PRE.
   destruct PRE as [MEMSAME EXECSAME].
+  rewrite <-MEMSAME, <-EXECSAME in *.
   step.
   step.
   step.
+  rewrite <-MEMSAME in *.
+  Ltac get_exec ::= 
+  repeat match goal with 
+  | [P: ?prop ?v |- _ ] => unfold prop in P
+  | [H: xbits (_ ?m) _ _ = _ |- context[N.testbit (update ?s _ _ ?m) _]] =>
+    rewrite (update_frame s _ _ m); try easy
+  | [H: xbits ?v ?l ?h = ?mem |- context[N.testbit ?v ?i]] =>
+    let HELP := fresh "H" in
+    assert (HELP: l <= i /\ N.succ i <= h) by (split; lia); clear HELP;
+    rewrite testbit_xbits, (xbits_split2 l i (N.succ i) h v mem);[reflexivity |lia..]
+  end; vm_compute (N.odd _); psimpl.
+Ltac effinv_none_hook ::= unfold effinv, effinv', p32_prog; get_exec.
+
+
+  eapply NIStep;
+   [ effinv_none_hook; reflexivity || fail_seek
+   | psa_some_hook; reflexivity || fail_seek
+   |  ].
+   
+   (* TODO: Continue here. ISA_step_and_simplify is hanging *)
+   (let c := fresh "c" in
+    let s := fresh "s" in
+    let x := fresh "x" in
+    let XS := fresh "XS" in
+    intros c s x XS).
+   Print ISA_step_and_simplify.
+   
+   Print step_stmt. Print exec_stmt.
+   Print populate_varlist.
+   Check fexec_stmt_init.
+   generalize XS. Check update_frame.
+(* Ltac mem_simpl := *)
+  repeat match goal with 
+  | [ |- context[getmem ?w ?e ?len (setmem ?w ?e ?len ?m ?a ?v) ?a]] => rewrite getmem_setmem
+  | [ |- _ ] => rewrite update_frame;[|intro;discriminate]
+  end.
+  Print overlap. Print N.min.
+  Print "<?". Print N.zeros.
+(* update_view updates the view of a memory from view1 of bits i to j-1 to
+   the view with bits x to y overwritten by the bits in val *)
+Definition update_view view i j val x y :=
+  if x <? i then
+    let view_shift = i - x in
+    view << view_shift .&
+Theorem update_mem:
+  forall w mem i j n a len v
+    (MEM: xbits mem (8*i) (8*j) = n)
+    (OV: overlap w i (j-i) a len)
+    (SMALL: a+len < 2 ^ w),
+    xbits (setmem w LittleE len mem a v) (8*(N.min i a)) (8*(N.max j (a+len)) =
+      v
+  rewrite update_frame.
+   mem_simpl.
+   eapply fexec_stmt_init in XS.
+   [ repeat
+      lazymatch type of XS
+      with
+      | exec_stmt _ (updstr (_[_ := _]) (List.rev _) vupdate) _ _ _ _ /\ _ =>
+          eapply fexec_stmt_updn in XS
+      end;
+      lazymatch type of XS
+      with
+      | exec_stmt ?c (updstr ?s (List.rev ?l) vupdate) ?q ?c' ?s' ?x /\ _ =>
+          let vs := eval compute in (other_vars_read l q) in
+          tacmap
+           ltac:(fun v =>
+                   try
+                    match goal with
+                    | SV:s v = ?n
+                      |- _ => eapply (fexec_stmt_hypn _ _ _ c s v n _ q c' s' x SV) in XS
+                    end) vs
+      end; eapply fexec_stmt_fin in XS
+   |  ]
+$
+  populate_varlist XS.
+  lazymatch type of XS with
+  | exec_stmt _ _ _ _ _ _ =>
+      populate_varlist XS;
+       [ step_precheck XS; eapply reduce_stmt in XS;
+          [ let unk := fresh "unknown" in
+            destruct XS as [unk XS]; compute in XS;
+             repeat
+              match type of XS with
+              | context [ unk ?i ] =>
+                  let n := fresh "n" in
+                  set (n := unk i) in XS; clearbody n
+              end; try clear unk
+          | reflexivity ]; cbv beta match delta [noe_setop noe_typop] in XS
+       | reflexivity ]
+  | _ => fail "Hypothesis is not of the form (exec_stmt ...)"
+  end.
+
+   (* step_stmt hangs *)
+   step_stmt XS. ; abstract_ignored_vars XS; psimpl_hyp XS; simpl_memaccs XS; destruct_memaccs XS;
+   try generalize_trace
+
+     ; ISA_step_and_simplify XS).
+     repeat
+      lazymatch type of XS with
+      | reset_temps _ s = _ /\ x = _ =>
+          try clear c; destruct XS as [XS ?]; subst x;
+           try
+            (let rt := fresh in
+             set (rt := reset_temps _ _)  at 1; psimpl_hyp rt; subst rt;
+              rewrite XS; clear XS; try clear s)
+      | exec_stmt _ _ (if ?c then _ else _) _ _ _ =>
+          let BC := fresh "BC" in
+          destruct c eqn:BC; ISA_step_and_simplify XS
+      | exec_stmt _ _ (N.iter _ _ _) _ _ _ => fail
+      | _ => ISA_step_and_simplify XS
+      end;
+     try
+      lazymatch goal with
+      | |- context [ exitof (?m + ?n) ] => simpl (m + n)
+      end; try (first [ rewrite exitof_none | rewrite exitof_some ])).
+   Print ISA_invseek.
+  eapply NIStep.
+  effinv_none_hook. 
+  
+  unfold invs, dynamicli_exit. effinv_none_hook.
+  
+  (p32_stmt (setmem 32 LittleE 4 (s V_MEM32) 12 12443) 12))
+
   (* Notice our address, 12, is exactly the location where we stored a 
      value, 12443, in memory. 12433 corresponds exactly to`PIL_li r5 777,`
      the instruction for loading the immediate 777 into register 5.
